add an opaque `model` flag, set to `false` for extraction

src/3d/prelude/EverParse3d.Readable.fst
@@ -7,32 +7,40 @@ module U32 = FStar.UInt32
 module G = FStar.Ghost
 module Seq = FStar.Seq
 
-let perm #t b = B.lbuffer (G.erased bool) (B.length b)
+module F = EverParse3d.Flags
+
+inline_for_extraction
+noextract
+let perm' (#t: Type0) (b: B.buffer t)
+: Tot Type0
+= B.lbuffer (G.erased bool) (B.length b)
+
+let perm #t b = if F.model then perm' b else unit
   
-let loc_perm #t #b p = B.loc_buffer p
+let loc_perm #t #b p = if F.model then B.loc_buffer (p <: perm' b) else B.loc_none
 
 let loc_perm_prop #t #b p = ()
 
 let valid_perm h #t #b p =
   B.live h b /\
   B.loc_buffer b `B.loc_disjoint` loc_perm p /\
-  B.live h p
+  (F.model ==> B.live h (p <: perm' b))
 
 let valid_perm_prop h #t #b p = ()
 
 let valid_perm_frame h #t #b p l h' = ()
 
-let perm_gsub #t #b p offset length = B.gsub p offset length
+let perm_gsub #t #b p offset length = if F.model then B.gsub (p <: perm' b) offset length else ()
 
-let perm_sub #t #b p offset length = B.sub p offset length
+let perm_sub #t #b p offset length = if F.model then B.sub (p <: perm' b) offset length else ()
 
-let perm_offset #t #b p offset = B.offset p offset
+let perm_offset #t #b p offset = if F.model then B.offset (p <: perm' b) offset else ()
 
 let perm_gsub_gsub #t #b p offset1 length1 offset2 length2 = ()
 
 let perm_gsub_zero_length #t #b p =
   B.gsub_zero_length b;
-  B.gsub_zero_length p
+  if F.model then B.gsub_zero_length (p <: perm' b)
 
 let loc_perm_gsub #t #b p offset length = ()
 
@@ -42,7 +50,7 @@ let loc_perm_from_to_disjoint #t #b p from1 to1 from2 to2 = ()
 
 let readable h #t #b p from to =
   valid_perm h p /\
-  B.as_seq h (B.gsub p from (to `U32.sub` from)) `Seq.equal` Seq.create (U32.v to - U32.v from) (G.hide true)
+  (F.model ==> B.as_seq h (B.gsub p from (to `U32.sub` from)) `Seq.equal` Seq.create (U32.v to - U32.v from) (G.hide true))
 
 let readable_prop h #t #b p from to = ()
 
@@ -50,19 +58,21 @@ let readable_gsub h #t #b p offset length from to = ()
 
 let readable_split h #t #b p from mid to =
   Seq.lemma_split (B.as_seq h (B.gsub b from (to `U32.sub` from))) (U32.v mid - U32.v from);
-  Seq.lemma_split (B.as_seq h (B.gsub p from (to `U32.sub` from))) (U32.v mid - U32.v from)
+  if F.model then Seq.lemma_split (B.as_seq h (B.gsub (p <: perm' b) from (to `U32.sub` from))) (U32.v mid - U32.v from)
 
 let readable_frame h #t #b p from to l h' = ()
 
 let unreadable h #t #b p from to =
-  valid_perm h p ==>
+  (valid_perm h p /\ F.model) ==>
   B.as_seq h (B.gsub p from (to `U32.sub` from)) `Seq.equal` Seq.create (U32.v to - U32.v from) (G.hide false)
 
 let unreadable_prop h #t #b p from to = ()
 
+let model = FStar.Ghost.hide F.model
+
 let readable_not_unreadable h #t #b p from to =
   let f () : Lemma
-    (requires (readable h p from to /\ unreadable h p from to))
+    (requires (F.model /\ readable h p from to /\ unreadable h p from to))
     (ensures False)
   = assert (valid_perm h p);
     let s = B.as_seq h (B.gsub p from (to `U32.sub` from)) in
@@ -78,11 +88,11 @@ let unreadable_gsub h #t #b p offset length from to = ()
 
 let unreadable_split h #t #b p from mid to =
   Seq.lemma_split (B.as_seq h (B.gsub b from (to `U32.sub` from))) (U32.v mid - U32.v from);
-  Seq.lemma_split (B.as_seq h (B.gsub p from (to `U32.sub` from))) (U32.v mid - U32.v from)
+  if F.model then Seq.lemma_split (B.as_seq h (B.gsub (p <: perm' b) from (to `U32.sub` from))) (U32.v mid - U32.v from)
 
 let unreadable_empty h #t #b p i = ()
 
 let unreadable_frame h #t #b p from to l h' = ()
 
 let scrub #t #b p from to =
-  B.fill (B.sub p from (to `U32.sub` from)) (G.hide false) (to `U32.sub` from)
+  if F.model then B.fill (B.sub (p <: perm' b) from (to `U32.sub` from)) (G.hide false) (to `U32.sub` from) else ()
