src/3d/prelude/EverParse3d.Flags.fst
@@ -1,0 +1,3 @@
+module EverParse3d.Flags
+
+let model = false
