src/3d/prelude/EverParse3d.Flags.fsti
@@ -1,0 +1,5 @@
+module EverParse3d.Flags
+
+inline_for_extraction
+noextract
+val model : bool
